%%% Local Variables:
%%% mode: latex
%%% TeX-master: "../index"
%%% End:

% Recommended:
% Show symmetric-key example with Alice-Bob diagram
% Mention modern algorithm (e.g. AES, Triple-DES)
% Benefits of public-key encryption (no key sharing)
% Show public-key example with RSA and Alice-Bob diagram

\subsection{Agenda}
\begin{enumerate}
\item Symmetric-key encryption
\item Symmetric- vs. public-key encryption
\item RSA
\end{enumerate}
\subsection*{RSA}
\begin{itemize}
\item Public key = (n,e) 
\item Private key = (p,q,d) where $ed \equiv 1 mod \phi (n)$.
\item Encryption is done by $Enc(m)= m^e mod n$.
\item Decryption is done by $Dec(c)=c^d mod n$.	
\item n = 2 primes p and q (pq=n)(big primes makes encryption safer)
\item e = is an integer $\in \mathbb{Z}^*_{\phi (n)}$, where $\phi (n)=(p-1)(q-1)$
\item d = is the multiplicative inverse of $e\; mod\;\phi (n)$
\end{itemize}
\subsubsection{Weakness}
\begin{itemize}
\item Attacker can get factors of n
\begin{itemize}
\item if attacker can factor n then he can find d same way that the system computes it
\end{itemize}
\item Attacker finds $\phi (n)$, then factors n
\begin{itemize}
\item if n is small attacker can setup an equation with two unknowns that uses $\phi (n)=(p-1)(q-1)$ since he knows $n=pq$
\begin{align*}
\phi (n)=n-p-q+1=>p&=n-\phi (n)-q+1\\
\mbox{since } p&=\frac{n}{q}\\
\frac{n}{q}&=n-\phi (n)-q+1\\
0&=q^2+q(\phi (n)-n-1)+n
\end{align*}
\end{itemize}
\item Attacker finds the decryption exponent d, then factors n
\begin{itemize}
\item If the attacker finds d its easy to factor n.
\end{itemize}
\item If $c_1$ and $c_2$ are encrypted with the same key then:
\begin{align*}
&(c_1c_2)^d\; mod\; n = (c_1^d) (c_2^d)\; mod \;n\\
&\mbox{which means}\\
&(c_1^d) (c_2^d)\; mod \;n = m_1m_2\;mod \; n
\end{align*}



\end{itemize}
\subsubsection{Example}
Alice and bob each have their individual private and public keys.
If alice wants to send an encrypted message to bob she needs his public key which she gets automatically.\\
Alice now encrypts her message $Enc(m)=m^e_{Bob}\;mod\;n_{Bob}$ and sends it to Bob. \\
Bob now has the ciphertext which needs to be decrypted. Since the message was encrypted with his public key his private key can decrypt it. $Dec(c_{Alice})=\;c^{d_{Bob}}_{Alice}\;mod\;n_{Bob}$.\\
Bob now gets Aliceâ€™s message.

\subsubsection{Proof}
\input{proofs/rsa.tex}